finishing verification

src/dice/HWAbstraction.fst
@@ -15,358 +15,81 @@ open FStar.Integers
 
 open DICE.Definitions
 
-type erased_pub_bytes (len:nat) = s:G.erased bytes_pub{
-  Seq.length (G.reveal s) == len
-}
+friend HWState
 
-type erased_sec_bytes (len:nat) = s:G.erased bytes_sec{
-  Seq.length (G.reveal s) == len
-}
-
-val uds_len : hashable_len
 let uds_len = 1ul
 
-val uds_bytes : erased_sec_bytes (v uds_len)
 let uds_bytes = G.hide (Seq.create (v uds_len) (I.u8 0))
 
-let pub_zero = I.uint #I.U8 #I.PUB 0
+let uds : b:IB.ibuffer byte_sec{
+  IB.frameOf b == HS.root /\
+  IB.recallable b /\
+  IB.length b == (v uds_len) /\
+  IB.value_is b uds_bytes} =
 
-val l0_image_header_size : signable_len
-let l0_image_header_size = 1ul
-
-val l0_image_header_bytes : erased_pub_bytes (v l0_image_header_size)
-let l0_image_header_bytes = G.hide (Seq.create (v l0_image_header_size) pub_zero)
-
-val l0_image_header_sig_bytes : erased_pub_bytes 64
-let l0_image_header_sig_bytes = G.hide (Seq.create 64 pub_zero)
-
-val l0_image_size : hashable_len
-let l0_image_size = 1ul
-
-val l0_image_bytes : erased_pub_bytes (v l0_image_size)
-let l0_image_bytes = G.hide (Seq.create (v l0_image_size) pub_zero)
-
-val l0_image_hash_bytes : erased_pub_bytes (v digest_len)
-let l0_image_hash_bytes = G.hide (Seq.create (v digest_len) pub_zero)
-
-val l0_auth_pubkey_bytes : erased_pub_bytes 32
-let l0_auth_pubkey_bytes = G.hide (Seq.create 32 pub_zero)
-
-type ibuffer_pub (len:nat) (s:erased_pub_bytes len) =
-  b:IB.ibuffer byte_pub{IB.recallable b /\ B.length b == len /\ IB.value_is b s}
-
-type ibuffer_sec (len:nat) (s:erased_sec_bytes len) =
-  b:IB.ibuffer byte_sec{IB.recallable b /\ B.length b == len /\ IB.value_is b s}
-
-noeq
-type l0_image_t = {
-  l0_image_header     : ibuffer_pub (v l0_image_header_size) l0_image_header_bytes;
-  l0_image_header_sig : ibuffer_pub 64 l0_image_header_sig_bytes;
-
-  l0_image            : ibuffer_pub (v l0_image_size) l0_image_bytes;
-  l0_image_hash       : ibuffer_pub (v digest_len) l0_image_hash_bytes;
-
-  l0_auth_pubkey      : ibuffer_pub 32 l0_auth_pubkey_bytes;
-}
-
-
-//not in the interface
-let l0_image : l0_image_t =
-  let l0_image_header = IB.igcmalloc HS.root pub_zero l0_image_header_size in
-  IB.witness_value l0_image_header;
-  let l0_image_header_sig = IB.igcmalloc HS.root pub_zero 64ul in
-  IB.witness_value l0_image_header_sig;
-  let l0_image = IB.igcmalloc HS.root pub_zero l0_image_size in
-  IB.witness_value l0_image;
-  let l0_image_hash = IB.igcmalloc HS.root pub_zero digest_len in
-  IB.witness_value l0_image_hash;
-  let l0_auth_pubkey = IB.igcmalloc HS.root pub_zero 32ul in
-  IB.witness_value l0_auth_pubkey;
-  { l0_image_header = l0_image_header;
-    l0_image_header_sig = l0_image_header_sig;
-    l0_image = l0_image;
-    l0_image_hash = l0_image_hash;
-    l0_auth_pubkey = l0_auth_pubkey }
-
-
-val get_l0_image (_:unit) : l0_image_t
-let get_l0_image _ = l0_image
-
-let uds : b:ibuffer_sec (v uds_len) uds_bytes{B.frameOf b == HS.root} =
   let uds = IB.igcmalloc HS.root (I.u8 0) uds_len in
   IB.witness_value uds;
   uds
 
-noeq
-type state = {
-  uds_enabled  : B.pointer bool;
-  stack_erased : B.pointer bool;
-  cdi : b:B.lbuffer byte_sec (v digest_len){
-    B.frameOf uds_enabled == HS.root /\
-    B.frameOf stack_erased == HS.root /\
-    B.frameOf b == HS.root /\
-    B.recallable uds_enabled /\
-    B.recallable stack_erased /\
-    B.recallable b /\
-    B.(all_disjoint [loc_buffer uds_enabled; loc_buffer stack_erased; loc_buffer b])
-  }
-}
+
+let l0_image_header_size = 1ul
+
+let l0_image_size = 1ul
 
 let st : state =
-  let uds_enabled = B.gcmalloc HS.root true 1ul in
-  let stack_erased = B.gcmalloc HS.root false 1ul in
+  let l0_image_header_size = 1ul in
+  let l0_binary_size = 1ul in
+  let ghost_state = B.gcmalloc HS.root (G.hide (true, true)) 1ul in
   let cdi = B.gcmalloc HS.root (I.u8 0) digest_len in
-  { uds_enabled = uds_enabled;
-    stack_erased = stack_erased;
-    cdi = cdi }
+  let l0_image_header = B.gcmalloc HS.root (I.u8 0) l0_image_header_size in
+  let l0_image_header_sig = B.gcmalloc HS.root (I.u8 0) 64ul in
+  let l0_binary = B.gcmalloc HS.root (I.u8 0) l0_binary_size in
+  let l0_binary_hash = B.gcmalloc HS.root (I.u8 0) digest_len in
+  let l0_image_auth_pubkey = B.gcmalloc HS.root (I.u8 0) 32ul in
 
+  let l0 = {
+    l0_image_header_size = l0_image_header_size;
+    l0_image_header = l0_image_header;
+    l0_image_header_sig = l0_image_header_sig;
+    l0_binary_size = l0_binary_size;
+    l0_binary = l0_binary;
+    l0_binary_hash = l0_binary_hash;
+    l0_image_auth_pubkey = l0_image_auth_pubkey
+  } in
 
-val uds_is_enabled (h:HS.mem) : Type0
-let uds_is_enabled h = b2t (B.get h st.uds_enabled 0)
+  { ghost_state = ghost_state;
+    cdi = cdi;
+    l0 = l0 }
 
-val stack_is_erased (h:HS.mem) : Type0
-let stack_is_erased h = b2t (B.get h st.stack_erased 0)
+let uds_is_enabled h = b2t (fst (B.get h st.ghost_state 0))
 
-val get_cdi_spec (_:unit) : B.lbuffer byte_sec (v digest_len)
-let get_cdi_spec () = st.cdi
+let stack_is_erased h = b2t (snd (B.get h st.ghost_state 0))
 
-val get_cdi (_:unit)
-  : Stack (B.lbuffer byte_sec (v digest_len))
-      (requires fun h -> True)
-      (ensures fun h0 b h1 ->
-        h0 == h1 /\
-        b == get_cdi_spec () /\
-        B.live h1 b)
-let get_cdi () =
-  B.recall st.cdi;
-  st.cdi
+let frame_ghost_state _ _ _ = ()
 
-val read_uds (uds_out:B.lbuffer byte_sec (v uds_len))
-  : Stack unit
-      (requires fun h ->
-        uds_is_enabled h /\
-        B.live h uds_out /\
-        HS.is_stack_region (B.frameOf uds_out))
-      (ensures fun h0 _ h1 ->
-        B.(modifies (loc_buffer uds_out) h0 h1) /\
-        B.as_seq h1 uds_out == G.reveal uds_bytes /\
-        uds_is_enabled h1 /\
-        B.as_seq h1 (get_cdi_spec ()) == B.as_seq h0 (get_cdi_spec ()))
 let read_uds uds_out =
   B.recall uds;
   IB.recall_value uds uds_bytes;
-  B.recall st.uds_enabled;
-  B.recall st.cdi;
   B.blit uds 0ul uds_out 0ul uds_len
 
-val disable_uds (_:unit)
-  : Stack unit
-      (requires fun h -> uds_is_enabled h)
-      (ensures fun h0 _ h1 ->
-        (~ (uds_is_enabled h1)) /\
-        B.as_seq h1 (get_cdi_spec ()) == B.as_seq h0 (get_cdi_spec ()))
 let disable_uds () =
-  B.recall st.uds_enabled;
-  B.recall st.cdi;
-  B.upd st.uds_enabled 0ul false
+  B.recall st.ghost_state;
+  let old_val = B.index st.ghost_state 0ul in
+  let new_val : (G.erased (bool & bool)) =
+    let (b1, b2) = G.reveal old_val in
+    G.hide (false, b2) in
+  B.upd st.ghost_state 0ul new_val
 
-val platform_zeroize_stack (_:unit)
-  : Stack unit
-      (requires fun h -> ~ (uds_is_enabled h))
-      (ensures fun h0 _ h1 ->
-        (~ (uds_is_enabled h1)) /\
-        stack_is_erased h1 /\
-        B.as_seq h1 (get_cdi_spec ()) == B.as_seq h0 (get_cdi_spec ()))
 let platform_zeroize_stack () =
-  B.recall st.uds_enabled;
-  B.recall st.stack_erased;
-  B.recall st.cdi;
-  B.upd st.stack_erased 0ul true
+  B.recall st.ghost_state;
+  let old_val = B.index st.ghost_state 0ul in
+  let new_val : (G.erased (bool & bool)) =
+    let (b1, b2) = G.reveal old_val in
+    G.hide (b1, true) in
+  B.upd st.ghost_state 0ul new_val
 
-
-
-
-// let uds_len = 0x20ul
-// let uds_value = fun _ -> Seq.create (v uds_len) (u8 0)
-// let uds_buf = IB.igcmalloc HS.root (u8 0) uds_len
-
-// let riot_pubkey_value = fun _ -> Seq.create 32 (u8 0)
-// let riot_pubkey_buf = IB.igcmalloc HS.root (u8 0) 32ul
-
-// let image_size = 1ul
-// let riot_image_value = fun _ -> Seq.create (v image_size) (u8 0)
-// let riot_image_buf = IB.igcmalloc HS.root (u8 0) image_size
-
-// let riot_image_hash_value = fun _ -> Seq.create 32 (u8 0)
-// let riot_image_hash_buf = IB.igcmalloc HS.root (u8 0) 32ul
-
-// let header_size = 100ul
-// let riot_image_header_value = fun _ -> Seq.create (v header_size) (u8 0)
-// let riot_image_header_buf = IB.igcmalloc HS.root (u8 0) header_size
-
-// let riot_header_sig_value = fun _ -> Seq.create 64 (u8 0)
-// let riot_header_sig_buf = IB.igcmalloc HS.root (u8 0) 64ul
-
-// #set-options "--__temp_no_proj HWAbstraction"
-
-// let stack_is_zeroized h =
-//   G.reveal (HS.sel h hwi_state) == Zeroized
-
-// let uds_is_disabled h =
-//   G.reveal (HS.sel h hwi_state) == Disabled
-
-// let get_riot_image () buf_disj
-// = (* Prf *) HST.recall hwi_state; (* Recall for disjointness *)
-//   let pubkey = B.alloca (u8 0x00) 32ul in
-//   // (* Prf *) let h = HST.get () in
-//   // (* Prf *) IB.recall riot_pubkey_buf;
-//   // (* Prf *) IB.recall_contents riot_pubkey_buf (Seq.create 32 (u8 0));
-//   // (* Prf *) IB.buffer_immutable_buffer_disjoint pubkey riot_pubkey_buf h;
-//   // B.blit riot_pubkey_buf 0ul pubkey 0ul 32ul;
-//   let image_base = B.alloca (u8 0x00) image_size in
-//   let image_hash = B.alloca (u8 0x00) 32ul in
-//   let image_header = B.alloca (u8 0x00) header_size in
-//   let header_sig = B.alloca (u8 0x00) 64ul in
-//   { header_size = header_size;
-//     image_header = image_header;
-//     image_hash = image_hash;
-//     header_sig = header_sig;
-//     image_size = image_size;
-//     image_base = image_base;
-//     pubkey = pubkey }
-
-// #push-options "--z3rlimit 16 --fuel 0 --ifuel 0"
-// let read_uds uds
-// = HST.recall hwi_state;
-//   HST.(hwi_state := Copied);
-//   B.fill uds (u8 0x00) uds_len
-// #pop-options
-
-// let platform_zeroize_stack ()
-// = HST.recall hwi_state;
-//   HST.(hwi_state := Zeroized)
-
-// let disable_uds ()
-// = HST.recall hwi_state;
-//   HST.(hwi_state := Disabled)
-//   // HST.witness_p local_state_ref uds_is_copied_predicate
-
-// let platform_zeroize len b
-// = B.fill b (u8 0) len;
-//   let h1 = HST.get () in
-//   Seq.lemma_split (B.as_seq h1 b) (v len)
-
-
-(* Old implemenations
-let initialize () =
-  HST.recall local_state_ref;
-  HST.(local_state_ref := Enabled);
-  HST.witness_p local_state_ref uds_is_initialized_predicate;
-
-  let uds = B.malloc HS.root (u8 0x00) uds_len in
-  let cdi = B.malloc HS.root (u8 0x00) cdi_len in
-
-  let binary_size = 1ul in
-  let header_sig = B.malloc HS.root (u8 0x00) 64ul in
-  let binary = B.malloc HS.root (u8 0x00) 1ul in
-  let pubkey = B.malloc HS.root (u8 0x00) 32ul in
-
-  let riot_header = {
-    binary_size = binary_size;
-    header_sig = header_sig;
-    binary = binary;
-    pubkey = pubkey
-  } in
-
-  let uds_seq =
-    let h = HST.get () in
-    G.hide (B.as_seq h uds) in
-
-  { uds = uds;
-    cdi = cdi;
-    riot_header = riot_header;
-    uds_val = uds_seq }
-
-let unset_uds st =
-  let uds = get_uds st in
-  B.fill uds (u8 0x00) uds_len;
-  let h = HST.get () in
-  assert (Seq.equal (B.as_seq h uds) (Seq.create (v uds_len) (u8 0x00)))
-
-let disable_uds st =
-  HST.recall_p local_state_ref uds_is_initialized_predicate;
-  HST.(local_state_ref := Disabled);
-  HST.witness_p local_state_ref uds_is_disabled_predicate;
-
-  B.free st.uds
-
-
-(* Old Implementation
-noeq
-type state = {
-  uds : B.buffer uint8;
-  cdi : B.buffer uint8;
-  riot_header : riot_header_t;
-  uds_val : s:G.erased (Seq.seq uint8){
-    B.length uds == v uds_len /\
-    B.length cdi == v cdi_len /\
-    Seq.length (G.reveal s) == v uds_len /\
-    B.freeable uds /\
-    B.freeable cdi /\
-    B.all_disjoint ([
-      B.loc_buffer uds;
-      B.loc_buffer cdi;
-      B.loc_mreference local_state_ref;
-      B.loc_buffer riot_header.header_sig;
-      B.loc_buffer riot_header.binary;
-      B.loc_buffer riot_header.pubkey])
-  };
-}
-
-
-let get_uds st = st.uds
-let get_cdi st = st.cdi
-let get_uds_value st = G.reveal st.uds_val
-let get_riot_header st = st.riot_header
-
-let initialize () =
-  HST.recall local_state_ref;
-  HST.(local_state_ref := Enabled);
-  HST.witness_p local_state_ref uds_is_initialized_predicate;
-
-  let uds = B.malloc HS.root (u8 0x00) uds_len in
-  let cdi = B.malloc HS.root (u8 0x00) cdi_len in
-
-  let binary_size = 1ul in
-  let header_sig = B.malloc HS.root (u8 0x00) 64ul in
-  let binary = B.malloc HS.root (u8 0x00) 1ul in
-  let pubkey = B.malloc HS.root (u8 0x00) 32ul in
-
-  let riot_header = {
-    binary_size = binary_size;
-    header_sig = header_sig;
-    binary = binary;
-    pubkey = pubkey
-  } in
-
-  let uds_seq =
-    let h = HST.get () in
-    G.hide (B.as_seq h uds) in
-
-  { uds = uds;
-    cdi = cdi;
-    riot_header = riot_header;
-    uds_val = uds_seq }
-
-let unset_uds st =
-  let uds = get_uds st in
-  B.fill uds (u8 0x00) uds_len;
-  let h = HST.get () in
-  assert (Seq.equal (B.as_seq h uds) (Seq.create (v uds_len) (u8 0x00)))
-
-let disable_uds st =
-  HST.recall_p local_state_ref uds_is_initialized_predicate;
-  HST.(local_state_ref := Disabled);
-  HST.witness_p local_state_ref uds_is_disabled_predicate;
-
-  B.free st.uds
+let platform_zeroize len b =
+  B.fill b (I.u8 0) len;
+  let h = get () in
+  assert (Seq.equal (Seq.slice (B.as_seq h b) 0 (UInt32.v len))
+                    (B.as_seq h b))
